case_study/cc_lean/Base.lean
@@ -1,1 +1,2 @@
 import Base.Big_Step
+import Base.Small_Step
