case_study/cc_lean/Base/Small_Step.lean
@@ -1,0 +1,112 @@
+import Definitions.Com
+import Base.Big_Step
+
+theorem small_step_deterministic : (cs ->> cs') -> (cs ->> cs'') -> (cs'' = cs') := by
+  intros h1 h2
+  induction h1 generalizing cs'' with
+    | var_assign x a s=> 
+      cases h2
+      rfl
+    | seq_1 c2 s => 
+      cases h2 with
+        | seq_1 => rfl
+        | seq_2 _ _ _ _ _ h => cases h
+    | seq_2 c1 c1' c2 s s' h ih => 
+      cases h2 with
+        | seq_1 => cases h
+        | seq_2 _ c2' _ _ s'' h' =>
+          have conf_eq: ((c1', s') = (c2', s'')) := by
+            symm; apply ih; assumption
+          rcases conf_eq
+          rfl
+    | if_true b c1 c2 s cond =>
+      cases h2 with
+        | if_true => rfl
+        | if_false _ _ _ _ cond' =>
+          rw [cond] at cond'
+          trivial
+    | if_false b c1 c2 s cond =>
+      cases h2 with
+        | if_true _ _ _ _ cond' =>
+          rw [cond'] at cond
+          trivial
+        | if_false _ _ _ _ cond' => rfl
+    | while_loop b c s =>
+      cases h2; rfl
+
+
+theorem small_seq_congr : ((c_1, s_1) ->* (c, s_2)) -> (c_1;;c_2, s_1) ->* (c;;c_2, s_2) := by
+  intros h
+  generalize rn : (c_1, s_1) = p1
+  generalize rn' : (c, s_2) = p2
+  rw [rn, rn'] at h
+  induction h generalizing c c_1 s_1 s_2 with
+    | refl => cases rn; cases rn'; apply RTC.refl
+    | tail cs cs' ht hh ih =>
+      cases rn; cases rn'
+      rcases cs with ⟨c1', s1'⟩ 
+      apply (RTC.tail (c1';;c_2, s1'))
+      apply ih <;> try rfl
+      apply SmallStep.seq_2
+      assumption
+
+theorem big_imp_small : (cs ==> t) -> (cs ->* (SKIP, t)) := by
+  intro h
+  induction h with
+    | skip s =>
+      apply RTC.refl
+    | assign =>
+      apply RTC_single
+      apply SmallStep.var_assign
+    | seq c1 c2 s t u h1 h2 ih ih' =>
+      have h_mid_1 : ((c1;;c2, s) ->* (SKIP;;c2, t)) := by
+        apply small_seq_congr
+        assumption
+      have h_mid_2 : ((SKIP;;c2, t) ->* (c2, t)) := by
+        apply RTC_single
+        apply SmallStep.seq_1
+      repeat (apply RTC_trans; assumption)
+      apply RTC.refl
+    | if_true b c c' s t hcond hb ih =>
+      have h: (RTC SmallStep (IF b THEN c ELSE c', s) (c, s)) := by
+        apply RTC_single
+        apply SmallStep.if_true
+        assumption
+      apply RTC_trans <;> assumption
+    | if_false b c c' s t hcond hb ih =>
+      have h: (RTC SmallStep (IF b THEN c ELSE c', s) (c', s)) := by
+        apply RTC_single
+        apply SmallStep.if_false
+        assumption
+      apply RTC_trans <;> assumption
+    | while_false cond d s' hcond => {
+      apply (RTC.tail (IF cond THEN d;;WHILE cond DO d ELSE SKIP, s'))
+      apply RTC_single
+      apply SmallStep.while_loop
+      apply SmallStep.if_false
+      assumption
+    }
+    | while_true cond d s' t' u hcond hb hr ih_c ih_r => {
+      have h1: (RTC SmallStep (WHILE cond DO d, s') (d;;WHILE cond DO d, s')) := by
+        have h2: (RTC SmallStep (WHILE cond DO d, s') (IF cond THEN d;;WHILE cond DO d ELSE SKIP, s')) := by
+          apply RTC_single
+          apply SmallStep.while_loop
+        apply RTC_trans
+        assumption
+        apply RTC_single
+        apply SmallStep.if_true
+        assumption
+
+      have h3: (RTC SmallStep (d;;WHILE cond DO d, s') (SKIP;;WHILE cond DO d, t') ) := by
+        apply small_seq_congr
+        assumption
+
+      have h4: (RTC SmallStep (SKIP;;WHILE cond DO d, t') (WHILE cond DO d, t') ) := by
+        apply RTC_single
+        apply SmallStep.seq_1
+
+      repeat (apply RTC_trans; assumption)
+      apply RTC.refl
+    }
+
+
